tuned whitespace;

src/Doc/Implementation/Prelim.thy
@@ -9,88 +9,78 @@ chapter \<open>Preliminaries\<close>
 section \<open>Contexts \label{sec:context}\<close>
 
 text \<open>
-  A logical context represents the background that is required for
-  formulating statements and composing proofs.  It acts as a medium to
-  produce formal content, depending on earlier material (declarations,
-  results etc.).
+  A logical context represents the background that is required for formulating
+  statements and composing proofs. It acts as a medium to produce formal
+  content, depending on earlier material (declarations, results etc.).
 
-  For example, derivations within the Isabelle/Pure logic can be
-  described as a judgment \<open>\<Gamma> \<turnstile>\<^sub>\<Theta> \<phi>\<close>, which means that a
-  proposition \<open>\<phi>\<close> is derivable from hypotheses \<open>\<Gamma>\<close>
-  within the theory \<open>\<Theta>\<close>.  There are logical reasons for
-  keeping \<open>\<Theta>\<close> and \<open>\<Gamma>\<close> separate: theories can be
-  liberal about supporting type constructors and schematic
-  polymorphism of constants and axioms, while the inner calculus of
-  \<open>\<Gamma> \<turnstile> \<phi>\<close> is strictly limited to Simple Type Theory (with
+  For example, derivations within the Isabelle/Pure logic can be described as
+  a judgment \<open>\<Gamma> \<turnstile>\<^sub>\<Theta> \<phi>\<close>, which means that a proposition \<open>\<phi>\<close> is derivable from
+  hypotheses \<open>\<Gamma>\<close> within the theory \<open>\<Theta>\<close>. There are logical reasons for keeping
+  \<open>\<Theta>\<close> and \<open>\<Gamma>\<close> separate: theories can be liberal about supporting type
+  constructors and schematic polymorphism of constants and axioms, while the
+  inner calculus of \<open>\<Gamma> \<turnstile> \<phi>\<close> is strictly limited to Simple Type Theory (with
   fixed type variables in the assumptions).
 
   \<^medskip>
-  Contexts and derivations are linked by the following key
-  principles:
+  Contexts and derivations are linked by the following key principles:
 
-  \<^item> Transfer: monotonicity of derivations admits results to be
-  transferred into a \<^emph>\<open>larger\<close> context, i.e.\ \<open>\<Gamma> \<turnstile>\<^sub>\<Theta>
-  \<phi>\<close> implies \<open>\<Gamma>' \<turnstile>\<^sub>\<Theta>\<^sub>' \<phi>\<close> for contexts \<open>\<Theta>'
-  \<supseteq> \<Theta>\<close> and \<open>\<Gamma>' \<supseteq> \<Gamma>\<close>.
+  \<^item> Transfer: monotonicity of derivations admits results to be transferred
+  into a \<^emph>\<open>larger\<close> context, i.e.\ \<open>\<Gamma> \<turnstile>\<^sub>\<Theta> \<phi>\<close> implies \<open>\<Gamma>' \<turnstile>\<^sub>\<Theta>\<^sub>' \<phi>\<close> for contexts
+  \<open>\<Theta>' \<supseteq> \<Theta>\<close> and \<open>\<Gamma>' \<supseteq> \<Gamma>\<close>.
 
-  \<^item> Export: discharge of hypotheses admits results to be exported
-  into a \<^emph>\<open>smaller\<close> context, i.e.\ \<open>\<Gamma>' \<turnstile>\<^sub>\<Theta> \<phi>\<close>
-  implies \<open>\<Gamma> \<turnstile>\<^sub>\<Theta> \<Delta> \<Longrightarrow> \<phi>\<close> where \<open>\<Gamma>' \<supseteq> \<Gamma>\<close> and
-  \<open>\<Delta> = \<Gamma>' - \<Gamma>\<close>.  Note that \<open>\<Theta>\<close> remains unchanged here,
-  only the \<open>\<Gamma>\<close> part is affected.
+  \<^item> Export: discharge of hypotheses admits results to be exported into a
+  \<^emph>\<open>smaller\<close> context, i.e.\ \<open>\<Gamma>' \<turnstile>\<^sub>\<Theta> \<phi>\<close> implies \<open>\<Gamma> \<turnstile>\<^sub>\<Theta> \<Delta> \<Longrightarrow> \<phi>\<close> where \<open>\<Gamma>' \<supseteq> \<Gamma>\<close>
+  and \<open>\<Delta> = \<Gamma>' - \<Gamma>\<close>. Note that \<open>\<Theta>\<close> remains unchanged here, only the \<open>\<Gamma>\<close> part is
+  affected.
 
 
   \<^medskip>
-  By modeling the main characteristics of the primitive
-  \<open>\<Theta>\<close> and \<open>\<Gamma>\<close> above, and abstracting over any
-  particular logical content, we arrive at the fundamental notions of
-  \<^emph>\<open>theory context\<close> and \<^emph>\<open>proof context\<close> in Isabelle/Isar.
-  These implement a certain policy to manage arbitrary \<^emph>\<open>context
-  data\<close>.  There is a strongly-typed mechanism to declare new kinds of
+  By modeling the main characteristics of the primitive \<open>\<Theta>\<close> and \<open>\<Gamma>\<close> above, and
+  abstracting over any particular logical content, we arrive at the
+  fundamental notions of \<^emph>\<open>theory context\<close> and \<^emph>\<open>proof context\<close> in
+  Isabelle/Isar. These implement a certain policy to manage arbitrary
+  \<^emph>\<open>context data\<close>. There is a strongly-typed mechanism to declare new kinds of
   data at compile time.
 
-  The internal bootstrap process of Isabelle/Pure eventually reaches a
-  stage where certain data slots provide the logical content of \<open>\<Theta>\<close> and \<open>\<Gamma>\<close> sketched above, but this does not stop there!
-  Various additional data slots support all kinds of mechanisms that
-  are not necessarily part of the core logic.
+  The internal bootstrap process of Isabelle/Pure eventually reaches a stage
+  where certain data slots provide the logical content of \<open>\<Theta>\<close> and \<open>\<Gamma>\<close> sketched
+  above, but this does not stop there! Various additional data slots support
+  all kinds of mechanisms that are not necessarily part of the core logic.
 
-  For example, there would be data for canonical introduction and
-  elimination rules for arbitrary operators (depending on the
-  object-logic and application), which enables users to perform
-  standard proof steps implicitly (cf.\ the \<open>rule\<close> method
-  @{cite "isabelle-isar-ref"}).
+  For example, there would be data for canonical introduction and elimination
+  rules for arbitrary operators (depending on the object-logic and
+  application), which enables users to perform standard proof steps implicitly
+  (cf.\ the \<open>rule\<close> method @{cite "isabelle-isar-ref"}).
 
   \<^medskip>
-  Thus Isabelle/Isar is able to bring forth more and more
-  concepts successively.  In particular, an object-logic like
-  Isabelle/HOL continues the Isabelle/Pure setup by adding specific
-  components for automated reasoning (classical reasoner, tableau
-  prover, structured induction etc.) and derived specification
-  mechanisms (inductive predicates, recursive functions etc.).  All of
-  this is ultimately based on the generic data management by theory
-  and proof contexts introduced here.
+  Thus Isabelle/Isar is able to bring forth more and more concepts
+  successively. In particular, an object-logic like Isabelle/HOL continues the
+  Isabelle/Pure setup by adding specific components for automated reasoning
+  (classical reasoner, tableau prover, structured induction etc.) and derived
+  specification mechanisms (inductive predicates, recursive functions etc.).
+  All of this is ultimately based on the generic data management by theory and
+  proof contexts introduced here.
 \<close>
 
 
 subsection \<open>Theory context \label{sec:context-theory}\<close>
 
-text \<open>A \<^emph>\<open>theory\<close> is a data container with explicit name and
-  unique identifier.  Theories are related by a (nominal) sub-theory
-  relation, which corresponds to the dependency graph of the original
-  construction; each theory is derived from a certain sub-graph of
-  ancestor theories.  To this end, the system maintains a set of
-  symbolic ``identification stamps'' within each theory.
+text \<open>
+  A \<^emph>\<open>theory\<close> is a data container with explicit name and unique identifier.
+  Theories are related by a (nominal) sub-theory relation, which corresponds
+  to the dependency graph of the original construction; each theory is derived
+  from a certain sub-graph of ancestor theories. To this end, the system
+  maintains a set of symbolic ``identification stamps'' within each theory.
 
-  The \<open>begin\<close> operation starts a new theory by importing several
-  parent theories (with merged contents) and entering a special mode of
-  nameless incremental updates, until the final \<open>end\<close> operation is
-  performed.
+  The \<open>begin\<close> operation starts a new theory by importing several parent
+  theories (with merged contents) and entering a special mode of nameless
+  incremental updates, until the final \<open>end\<close> operation is performed.
 
   \<^medskip>
-  The example in \figref{fig:ex-theory} below shows a theory
-  graph derived from \<open>Pure\<close>, with theory \<open>Length\<close>
-  importing \<open>Nat\<close> and \<open>List\<close>.  The body of \<open>Length\<close> consists of a sequence of updates, resulting in locally a
-  linear sub-theory relation for each intermediate step.
+  The example in \figref{fig:ex-theory} below shows a theory graph derived
+  from \<open>Pure\<close>, with theory \<open>Length\<close> importing \<open>Nat\<close> and \<open>List\<close>. The body of
+  \<open>Length\<close> consists of a sequence of updates, resulting in locally a linear
+  sub-theory relation for each intermediate step.
 
   \begin{figure}[htb]
   \begin{center}
@@ -111,10 +101,10 @@ text \<open>A \<^emph>\<open>theory\<close> is a data container with explicit na
   \end{figure}
 
   \<^medskip>
-  Derived formal entities may retain a reference to the
-  background theory in order to indicate the formal context from which
-  they were produced.  This provides an immutable certificate of the
-  background theory.\<close>
+  Derived formal entities may retain a reference to the background theory in
+  order to indicate the formal context from which they were produced. This
+  provides an immutable certificate of the background theory.
+\<close>
 
 text %mlref \<open>
   \begin{mldecls}
@@ -128,24 +118,21 @@ text %mlref \<open>
 
   \<^descr> Type @{ML_type theory} represents theory contexts.
 
-  \<^descr> @{ML "Context.eq_thy"}~\<open>(thy\<^sub>1, thy\<^sub>2)\<close> check strict
-  identity of two theories.
+  \<^descr> @{ML "Context.eq_thy"}~\<open>(thy\<^sub>1, thy\<^sub>2)\<close> check strict identity of two
+  theories.
 
-  \<^descr> @{ML "Context.subthy"}~\<open>(thy\<^sub>1, thy\<^sub>2)\<close> compares theories
-  according to the intrinsic graph structure of the construction.
-  This sub-theory relation is a nominal approximation of inclusion
-  (\<open>\<subseteq>\<close>) of the corresponding content (according to the
-  semantics of the ML modules that implement the data).
+  \<^descr> @{ML "Context.subthy"}~\<open>(thy\<^sub>1, thy\<^sub>2)\<close> compares theories according to the
+  intrinsic graph structure of the construction. This sub-theory relation is a
+  nominal approximation of inclusion (\<open>\<subseteq>\<close>) of the corresponding content
+  (according to the semantics of the ML modules that implement the data).
 
-  \<^descr> @{ML "Theory.begin_theory"}~\<open>name parents\<close> constructs
-  a new theory based on the given parents.  This ML function is
-  normally not invoked directly.
+  \<^descr> @{ML "Theory.begin_theory"}~\<open>name parents\<close> constructs a new theory based
+  on the given parents. This ML function is normally not invoked directly.
 
-  \<^descr> @{ML "Theory.parents_of"}~\<open>thy\<close> returns the direct
-  ancestors of \<open>thy\<close>.
+  \<^descr> @{ML "Theory.parents_of"}~\<open>thy\<close> returns the direct ancestors of \<open>thy\<close>.
 
-  \<^descr> @{ML "Theory.ancestors_of"}~\<open>thy\<close> returns all
-  ancestors of \<open>thy\<close> (not including \<open>thy\<close> itself).
+  \<^descr> @{ML "Theory.ancestors_of"}~\<open>thy\<close> returns all ancestors of \<open>thy\<close> (not
+  including \<open>thy\<close> itself).
 \<close>
 
 text %mlantiq \<open>
@@ -160,45 +147,43 @@ text %mlantiq \<open>
   @@{ML_antiquotation theory_context} nameref
   \<close>}
 
-  \<^descr> \<open>@{theory}\<close> refers to the background theory of the
-  current context --- as abstract value.
+  \<^descr> \<open>@{theory}\<close> refers to the background theory of the current context --- as
+  abstract value.
 
-  \<^descr> \<open>@{theory A}\<close> refers to an explicitly named ancestor
-  theory \<open>A\<close> of the background theory of the current context
-  --- as abstract value.
+  \<^descr> \<open>@{theory A}\<close> refers to an explicitly named ancestor theory \<open>A\<close> of the
+  background theory of the current context --- as abstract value.
 
-  \<^descr> \<open>@{theory_context A}\<close> is similar to \<open>@{theory
-  A}\<close>, but presents the result as initial @{ML_type Proof.context}
-  (see also @{ML Proof_Context.init_global}).
+  \<^descr> \<open>@{theory_context A}\<close> is similar to \<open>@{theory A}\<close>, but presents the result
+  as initial @{ML_type Proof.context} (see also @{ML
+  Proof_Context.init_global}).
 \<close>
 
 
 subsection \<open>Proof context \label{sec:context-proof}\<close>
 
-text \<open>A proof context is a container for pure data that refers to
-  the theory from which it is derived. The \<open>init\<close> operation
-  creates a proof context from a given theory. There is an explicit
-  \<open>transfer\<close> operation to force resynchronization with updates
-  to the background theory -- this is rarely required in practice.
+text \<open>
+  A proof context is a container for pure data that refers to the theory from
+  which it is derived. The \<open>init\<close> operation creates a proof context from a
+  given theory. There is an explicit \<open>transfer\<close> operation to force
+  resynchronization with updates to the background theory -- this is rarely
+  required in practice.
 
-  Entities derived in a proof context need to record logical
-  requirements explicitly, since there is no separate context
-  identification or symbolic inclusion as for theories.  For example,
-  hypotheses used in primitive derivations (cf.\ \secref{sec:thms})
-  are recorded separately within the sequent \<open>\<Gamma> \<turnstile> \<phi>\<close>, just to
-  make double sure.  Results could still leak into an alien proof
-  context due to programming errors, but Isabelle/Isar includes some
-  extra validity checks in critical positions, notably at the end of a
+  Entities derived in a proof context need to record logical requirements
+  explicitly, since there is no separate context identification or symbolic
+  inclusion as for theories. For example, hypotheses used in primitive
+  derivations (cf.\ \secref{sec:thms}) are recorded separately within the
+  sequent \<open>\<Gamma> \<turnstile> \<phi>\<close>, just to make double sure. Results could still leak into an
+  alien proof context due to programming errors, but Isabelle/Isar includes
+  some extra validity checks in critical positions, notably at the end of a
   sub-proof.
 
   Proof contexts may be manipulated arbitrarily, although the common
-  discipline is to follow block structure as a mental model: a given
-  context is extended consecutively, and results are exported back
-  into the original context.  Note that an Isar proof state models
-  block-structured reasoning explicitly, using a stack of proof
-  contexts internally.  For various technical reasons, the background
-  theory of an Isar proof state must not be changed while the proof is
-  still under construction!
+  discipline is to follow block structure as a mental model: a given context
+  is extended consecutively, and results are exported back into the original
+  context. Note that an Isar proof state models block-structured reasoning
+  explicitly, using a stack of proof contexts internally. For various
+  technical reasons, the background theory of an Isar proof state must not be
+  changed while the proof is still under construction!
 \<close>
 
 text %mlref \<open>
@@ -211,14 +196,14 @@ text %mlref \<open>
 
   \<^descr> Type @{ML_type Proof.context} represents proof contexts.
 
-  \<^descr> @{ML Proof_Context.init_global}~\<open>thy\<close> produces a proof
-  context derived from \<open>thy\<close>, initializing all data.
+  \<^descr> @{ML Proof_Context.init_global}~\<open>thy\<close> produces a proof context derived
+  from \<open>thy\<close>, initializing all data.
 
-  \<^descr> @{ML Proof_Context.theory_of}~\<open>ctxt\<close> selects the
-  background theory from \<open>ctxt\<close>.
+  \<^descr> @{ML Proof_Context.theory_of}~\<open>ctxt\<close> selects the background theory from
+  \<open>ctxt\<close>.
 
-  \<^descr> @{ML Proof_Context.transfer}~\<open>thy ctxt\<close> promotes the
-  background theory of \<open>ctxt\<close> to the super theory \<open>thy\<close>.
+  \<^descr> @{ML Proof_Context.transfer}~\<open>thy ctxt\<close> promotes the background theory of
+  \<open>ctxt\<close> to the super theory \<open>thy\<close>.
 \<close>
 
 text %mlantiq \<open>
@@ -226,9 +211,9 @@ text %mlantiq \<open>
   @{ML_antiquotation_def "context"} & : & \<open>ML_antiquotation\<close> \\
   \end{matharray}
 
-  \<^descr> \<open>@{context}\<close> refers to \<^emph>\<open>the\<close> context at
-  compile-time --- as abstract value.  Independently of (local) theory
-  or proof mode, this always produces a meaningful result.
+  \<^descr> \<open>@{context}\<close> refers to \<^emph>\<open>the\<close> context at compile-time --- as abstract
+  value. Independently of (local) theory or proof mode, this always produces a
+  meaningful result.
 
   This is probably the most common antiquotation in interactive
   experimentation with ML inside Isar.
@@ -238,17 +223,16 @@ text %mlantiq \<open>
 subsection \<open>Generic contexts \label{sec:generic-context}\<close>
 
 text \<open>
-  A generic context is the disjoint sum of either a theory or proof
-  context.  Occasionally, this enables uniform treatment of generic
-  context data, typically extra-logical information.  Operations on
-  generic contexts include the usual injections, partial selections,
-  and combinators for lifting operations on either component of the
-  disjoint sum.
+  A generic context is the disjoint sum of either a theory or proof context.
+  Occasionally, this enables uniform treatment of generic context data,
+  typically extra-logical information. Operations on generic contexts include
+  the usual injections, partial selections, and combinators for lifting
+  operations on either component of the disjoint sum.
 
-  Moreover, there are total operations \<open>theory_of\<close> and \<open>proof_of\<close> to convert a generic context into either kind: a theory
-  can always be selected from the sum, while a proof context might
-  have to be constructed by an ad-hoc \<open>init\<close> operation, which
-  incurs a small runtime overhead.
+  Moreover, there are total operations \<open>theory_of\<close> and \<open>proof_of\<close> to convert a
+  generic context into either kind: a theory can always be selected from the
+  sum, while a proof context might have to be constructed by an ad-hoc \<open>init\<close>
+  operation, which incurs a small runtime overhead.
 \<close>
 
 text %mlref \<open>
@@ -258,27 +242,27 @@ text %mlref \<open>
   @{index_ML Context.proof_of: "Context.generic -> Proof.context"} \\
   \end{mldecls}
 
-  \<^descr> Type @{ML_type Context.generic} is the direct sum of @{ML_type
-  "theory"} and @{ML_type "Proof.context"}, with the datatype
-  constructors @{ML "Context.Theory"} and @{ML "Context.Proof"}.
+  \<^descr> Type @{ML_type Context.generic} is the direct sum of @{ML_type "theory"}
+  and @{ML_type "Proof.context"}, with the datatype constructors @{ML
+  "Context.Theory"} and @{ML "Context.Proof"}.
 
-  \<^descr> @{ML Context.theory_of}~\<open>context\<close> always produces a
-  theory from the generic \<open>context\<close>, using @{ML
-  "Proof_Context.theory_of"} as required.
+  \<^descr> @{ML Context.theory_of}~\<open>context\<close> always produces a theory from the
+  generic \<open>context\<close>, using @{ML "Proof_Context.theory_of"} as required.
 
-  \<^descr> @{ML Context.proof_of}~\<open>context\<close> always produces a
-  proof context from the generic \<open>context\<close>, using @{ML
-  "Proof_Context.init_global"} as required (note that this re-initializes the
-  context data with each invocation).
+  \<^descr> @{ML Context.proof_of}~\<open>context\<close> always produces a proof context from the
+  generic \<open>context\<close>, using @{ML "Proof_Context.init_global"} as required (note
+  that this re-initializes the context data with each invocation).
 \<close>
 
 
 subsection \<open>Context data \label{sec:context-data}\<close>
 
-text \<open>The main purpose of theory and proof contexts is to manage
-  arbitrary (pure) data.  New data types can be declared incrementally
-  at compile time.  There are separate declaration mechanisms for any
-  of the three kinds of contexts: theory, proof, generic.\<close>
+text \<open>
+  The main purpose of theory and proof contexts is to manage arbitrary (pure)
+  data. New data types can be declared incrementally at compile time. There
+  are separate declaration mechanisms for any of the three kinds of contexts:
+  theory, proof, generic.
+\<close>
 
 paragraph \<open>Theory data\<close>
 text \<open>declarations need to implement the following ML signature:
@@ -292,18 +276,18 @@ text \<open>declarations need to implement the following ML signature:
   \end{tabular}
   \<^medskip>
 
-  The \<open>empty\<close> value acts as initial default for \<^emph>\<open>any\<close>
-  theory that does not declare actual data content; \<open>extend\<close>
-  is acts like a unitary version of \<open>merge\<close>.
+  The \<open>empty\<close> value acts as initial default for \<^emph>\<open>any\<close> theory that does not
+  declare actual data content; \<open>extend\<close> is acts like a unitary version of
+  \<open>merge\<close>.
 
-  Implementing \<open>merge\<close> can be tricky.  The general idea is
-  that \<open>merge (data\<^sub>1, data\<^sub>2)\<close> inserts those parts of \<open>data\<^sub>2\<close> into \<open>data\<^sub>1\<close> that are not yet present, while
-  keeping the general order of things.  The @{ML Library.merge}
+  Implementing \<open>merge\<close> can be tricky. The general idea is that \<open>merge (data\<^sub>1,
+  data\<^sub>2)\<close> inserts those parts of \<open>data\<^sub>2\<close> into \<open>data\<^sub>1\<close> that are not yet
+  present, while keeping the general order of things. The @{ML Library.merge}
   function on plain lists may serve as canonical template.
 
-  Particularly note that shared parts of the data must not be
-  duplicated by naive concatenation, or a theory graph that is like a
-  chain of diamonds would cause an exponential blowup!
+  Particularly note that shared parts of the data must not be duplicated by
+  naive concatenation, or a theory graph that is like a chain of diamonds
+  would cause an exponential blowup!
 \<close>
 
 paragraph \<open>Proof context data\<close>
@@ -316,26 +300,25 @@ text \<open>declarations need to implement the following ML signature:
   \end{tabular}
   \<^medskip>
 
-  The \<open>init\<close> operation is supposed to produce a pure value
-  from the given background theory and should be somehow
-  ``immediate''.  Whenever a proof context is initialized, which
-  happens frequently, the the system invokes the \<open>init\<close>
-  operation of \<^emph>\<open>all\<close> theory data slots ever declared.  This also
-  means that one needs to be economic about the total number of proof
-  data declarations in the system, i.e.\ each ML module should declare
-  at most one, sometimes two data slots for its internal use.
-  Repeated data declarations to simulate a record type should be
-  avoided!
+  The \<open>init\<close> operation is supposed to produce a pure value from the given
+  background theory and should be somehow ``immediate''. Whenever a proof
+  context is initialized, which happens frequently, the the system invokes the
+  \<open>init\<close> operation of \<^emph>\<open>all\<close> theory data slots ever declared. This also means
+  that one needs to be economic about the total number of proof data
+  declarations in the system, i.e.\ each ML module should declare at most one,
+  sometimes two data slots for its internal use. Repeated data declarations to
+  simulate a record type should be avoided!
 \<close>
 
 paragraph \<open>Generic data\<close>
-text \<open>provides a hybrid interface for both theory and proof data. The \<open>init\<close>
-  operation for proof contexts is predefined to select the current data
-  value from the background theory.
+text \<open>
+  provides a hybrid interface for both theory and proof data. The \<open>init\<close>
+  operation for proof contexts is predefined to select the current data value
+  from the background theory.
 
   \<^bigskip>
-  Any of the above data declarations over type \<open>T\<close>
-  result in an ML structure with the following signature:
+  Any of the above data declarations over type \<open>T\<close> result in an ML structure
+  with the following signature:
 
   \<^medskip>
   \begin{tabular}{ll}
@@ -345,12 +328,12 @@ text \<open>provides a hybrid interface for both theory and proof data. The \<op
   \end{tabular}
   \<^medskip>
 
-  These other operations provide exclusive access for the particular
-  kind of context (theory, proof, or generic context).  This interface
-  observes the ML discipline for types and scopes: there is no other
-  way to access the corresponding data slot of a context.  By keeping
-  these operations private, an Isabelle/ML module may maintain
-  abstract values authentically.\<close>
+  These other operations provide exclusive access for the particular kind of
+  context (theory, proof, or generic context). This interface observes the ML
+  discipline for types and scopes: there is no other way to access the
+  corresponding data slot of a context. By keeping these operations private,
+  an Isabelle/ML module may maintain abstract values authentically.
+\<close>
 
 text %mlref \<open>
   \begin{mldecls}
@@ -359,22 +342,20 @@ text %mlref \<open>
   @{index_ML_functor Generic_Data} \\
   \end{mldecls}
 
-  \<^descr> @{ML_functor Theory_Data}\<open>(spec)\<close> declares data for
-  type @{ML_type theory} according to the specification provided as
-  argument structure.  The resulting structure provides data init and
-  access operations as described above.
+  \<^descr> @{ML_functor Theory_Data}\<open>(spec)\<close> declares data for type @{ML_type theory}
+  according to the specification provided as argument structure. The resulting
+  structure provides data init and access operations as described above.
 
-  \<^descr> @{ML_functor Proof_Data}\<open>(spec)\<close> is analogous to
-  @{ML_functor Theory_Data} for type @{ML_type Proof.context}.
+  \<^descr> @{ML_functor Proof_Data}\<open>(spec)\<close> is analogous to @{ML_functor Theory_Data}
+  for type @{ML_type Proof.context}.
 
-  \<^descr> @{ML_functor Generic_Data}\<open>(spec)\<close> is analogous to
-  @{ML_functor Theory_Data} for type @{ML_type Context.generic}.
-\<close>
+  \<^descr> @{ML_functor Generic_Data}\<open>(spec)\<close> is analogous to @{ML_functor
+  Theory_Data} for type @{ML_type Context.generic}. \<close>
 
 text %mlex \<open>
-  The following artificial example demonstrates theory
-  data: we maintain a set of terms that are supposed to be wellformed
-  wrt.\ the enclosing theory.  The public interface is as follows:
+  The following artificial example demonstrates theory data: we maintain a set
+  of terms that are supposed to be wellformed wrt.\ the enclosing theory. The
+  public interface is as follows:
 \<close>
 
 ML \<open>
@@ -385,9 +366,10 @@ ML \<open>
   end;
 \<close>
 
-text \<open>The implementation uses private theory data internally, and
-  only exposes an operation that involves explicit argument checking
-  wrt.\ the given theory.\<close>
+text \<open>
+  The implementation uses private theory data internally, and only exposes an
+  operation that involves explicit argument checking wrt.\ the given theory.
+\<close>
 
 ML \<open>
   structure Wellformed_Terms: WELLFORMED_TERMS =
@@ -414,59 +396,57 @@ ML \<open>
   end;
 \<close>
 
-text \<open>Type @{ML_type "term Ord_List.T"} is used for reasonably
-  efficient representation of a set of terms: all operations are
-  linear in the number of stored elements.  Here we assume that users
-  of this module do not care about the declaration order, since that
-  data structure forces its own arrangement of elements.
+text \<open>
+  Type @{ML_type "term Ord_List.T"} is used for reasonably efficient
+  representation of a set of terms: all operations are linear in the number of
+  stored elements. Here we assume that users of this module do not care about
+  the declaration order, since that data structure forces its own arrangement
+  of elements.
 
-  Observe how the @{ML_text merge} operation joins the data slots of
-  the two constituents: @{ML Ord_List.union} prevents duplication of
-  common data from different branches, thus avoiding the danger of
-  exponential blowup.  Plain list append etc.\ must never be used for
-  theory data merges!
+  Observe how the @{ML_text merge} operation joins the data slots of the two
+  constituents: @{ML Ord_List.union} prevents duplication of common data from
+  different branches, thus avoiding the danger of exponential blowup. Plain
+  list append etc.\ must never be used for theory data merges!
 
   \<^medskip>
   Our intended invariant is achieved as follows:
 
-  \<^enum> @{ML Wellformed_Terms.add} only admits terms that have passed
-  the @{ML Sign.cert_term} check of the given theory at that point.
+    \<^enum> @{ML Wellformed_Terms.add} only admits terms that have passed the @{ML
+    Sign.cert_term} check of the given theory at that point.
+  
+    \<^enum> Wellformedness in the sense of @{ML Sign.cert_term} is monotonic wrt.\
+    the sub-theory relation. So our data can move upwards in the hierarchy
+    (via extension or merges), and maintain wellformedness without further
+    checks.
 
-  \<^enum> Wellformedness in the sense of @{ML Sign.cert_term} is
-  monotonic wrt.\ the sub-theory relation.  So our data can move
-  upwards in the hierarchy (via extension or merges), and maintain
-  wellformedness without further checks.
+  Note that all basic operations of the inference kernel (which includes @{ML
+  Sign.cert_term}) observe this monotonicity principle, but other user-space
+  tools don't. For example, fully-featured type-inference via @{ML
+  Syntax.check_term} (cf.\ \secref{sec:term-check}) is not necessarily
+  monotonic wrt.\ the background theory, since constraints of term constants
+  can be modified by later declarations, for example.
 
-
-  Note that all basic operations of the inference kernel (which
-  includes @{ML Sign.cert_term}) observe this monotonicity principle,
-  but other user-space tools don't.  For example, fully-featured
-  type-inference via @{ML Syntax.check_term} (cf.\
-  \secref{sec:term-check}) is not necessarily monotonic wrt.\ the
-  background theory, since constraints of term constants can be
-  modified by later declarations, for example.
-
-  In most cases, user-space context data does not have to take such
-  invariants too seriously.  The situation is different in the
-  implementation of the inference kernel itself, which uses the very
-  same data mechanisms for types, constants, axioms etc.
+  In most cases, user-space context data does not have to take such invariants
+  too seriously. The situation is different in the implementation of the
+  inference kernel itself, which uses the very same data mechanisms for types,
+  constants, axioms etc.
 \<close>
 
 
 subsection \<open>Configuration options \label{sec:config-options}\<close>
 
-text \<open>A \<^emph>\<open>configuration option\<close> is a named optional value of
-  some basic type (Boolean, integer, string) that is stored in the
-  context.  It is a simple application of general context data
-  (\secref{sec:context-data}) that is sufficiently common to justify
-  customized setup, which includes some concrete declarations for
-  end-users using existing notation for attributes (cf.\
-  \secref{sec:attributes}).
+text \<open>
+  A \<^emph>\<open>configuration option\<close> is a named optional value of some basic type
+  (Boolean, integer, string) that is stored in the context. It is a simple
+  application of general context data (\secref{sec:context-data}) that is
+  sufficiently common to justify customized setup, which includes some
+  concrete declarations for end-users using existing notation for attributes
+  (cf.\ \secref{sec:attributes}).
 
-  For example, the predefined configuration option @{attribute
-  show_types} controls output of explicit type constraints for
-  variables in printed terms (cf.\ \secref{sec:read-print}).  Its
-  value can be modified within Isar text like this:
+  For example, the predefined configuration option @{attribute show_types}
+  controls output of explicit type constraints for variables in printed terms
+  (cf.\ \secref{sec:read-print}). Its value can be modified within Isar text
+  like this:
 \<close>
 
 experiment
@@ -489,16 +469,18 @@ end
 
 end
 
-text \<open>Configuration options that are not set explicitly hold a
-  default value that can depend on the application context.  This
-  allows to retrieve the value from another slot within the context,
-  or fall back on a global preference mechanism, for example.
+text \<open>
+  Configuration options that are not set explicitly hold a default value that
+  can depend on the application context. This allows to retrieve the value
+  from another slot within the context, or fall back on a global preference
+  mechanism, for example.
 
-  The operations to declare configuration options and get/map their
-  values are modeled as direct replacements for historic global
-  references, only that the context is made explicit.  This allows
-  easy configuration of tools, without relying on the execution order
-  as required for old-style mutable references.\<close>
+  The operations to declare configuration options and get/map their values are
+  modeled as direct replacements for historic global references, only that the
+  context is made explicit. This allows easy configuration of tools, without
+  relying on the execution order as required for old-style mutable
+  references.
+\<close>
 
 text %mlref \<open>
   \begin{mldecls}
@@ -514,37 +496,38 @@ text %mlref \<open>
   string Config.T"} \\
   \end{mldecls}
 
-  \<^descr> @{ML Config.get}~\<open>ctxt config\<close> gets the value of
-  \<open>config\<close> in the given context.
+  \<^descr> @{ML Config.get}~\<open>ctxt config\<close> gets the value of \<open>config\<close> in the given
+  context.
 
-  \<^descr> @{ML Config.map}~\<open>config f ctxt\<close> updates the context
-  by updating the value of \<open>config\<close>.
+  \<^descr> @{ML Config.map}~\<open>config f ctxt\<close> updates the context by updating the value
+  of \<open>config\<close>.
 
-  \<^descr> \<open>config =\<close>~@{ML Attrib.setup_config_bool}~\<open>name
-  default\<close> creates a named configuration option of type @{ML_type
-  bool}, with the given \<open>default\<close> depending on the application
-  context.  The resulting \<open>config\<close> can be used to get/map its
-  value in a given context.  There is an implicit update of the
-  background theory that registers the option as attribute with some
-  concrete syntax.
+  \<^descr> \<open>config =\<close>~@{ML Attrib.setup_config_bool}~\<open>name default\<close> creates a named
+  configuration option of type @{ML_type bool}, with the given \<open>default\<close>
+  depending on the application context. The resulting \<open>config\<close> can be used to
+  get/map its value in a given context. There is an implicit update of the
+  background theory that registers the option as attribute with some concrete
+  syntax.
 
   \<^descr> @{ML Attrib.config_int}, @{ML Attrib.config_real}, and @{ML
-  Attrib.config_string} work like @{ML Attrib.config_bool}, but for
-  types @{ML_type int} and @{ML_type string}, respectively.
+  Attrib.config_string} work like @{ML Attrib.config_bool}, but for types
+  @{ML_type int} and @{ML_type string}, respectively.
 \<close>
 
-text %mlex \<open>The following example shows how to declare and use a
-  Boolean configuration option called \<open>my_flag\<close> with constant
-  default value @{ML false}.\<close>
+text %mlex \<open>
+  The following example shows how to declare and use a Boolean configuration
+  option called \<open>my_flag\<close> with constant default value @{ML false}.
+\<close>
 
 ML \<open>
   val my_flag =
     Attrib.setup_config_bool @{binding my_flag} (K false)
 \<close>
 
-text \<open>Now the user can refer to @{attribute my_flag} in
-  declarations, while ML tools can retrieve the current value from the
-  context via @{ML Config.get}.\<close>
+text \<open>
+  Now the user can refer to @{attribute my_flag} in declarations, while ML
+  tools can retrieve the current value from the context via @{ML Config.get}.
+\<close>
 
 ML_val \<open>@{assert} (Config.get @{context} my_flag = false)\<close>
 
@@ -561,8 +544,10 @@ begin
   ML_val \<open>@{assert} (Config.get @{context} my_flag = true)\<close>
 end
 
-text \<open>Here is another example involving ML type @{ML_type real}
-  (floating-point numbers).\<close>
+text \<open>
+  Here is another example involving ML type @{ML_type real} (floating-point
+  numbers).
+\<close>
 
 ML \<open>
   val airspeed_velocity =
@@ -575,62 +560,58 @@ declare [[airspeed_velocity = 9.9]]
 
 section \<open>Names \label{sec:names}\<close>
 
-text \<open>In principle, a name is just a string, but there are various
-  conventions for representing additional structure.  For example,
-  ``\<open>Foo.bar.baz\<close>'' is considered as a long name consisting of
-  qualifier \<open>Foo.bar\<close> and base name \<open>baz\<close>.  The
-  individual constituents of a name may have further substructure,
-  e.g.\ the string ``\<^verbatim>\<open>\<alpha>\<close>'' encodes as a single
-  symbol (\secref{sec:symbols}).
+text \<open>
+  In principle, a name is just a string, but there are various conventions for
+  representing additional structure. For example, ``\<open>Foo.bar.baz\<close>'' is
+  considered as a long name consisting of qualifier \<open>Foo.bar\<close> and base name
+  \<open>baz\<close>. The individual constituents of a name may have further substructure,
+  e.g.\ the string ``\<^verbatim>\<open>\<alpha>\<close>'' encodes as a single symbol (\secref{sec:symbols}).
 
   \<^medskip>
-  Subsequently, we shall introduce specific categories of
-  names.  Roughly speaking these correspond to logical entities as
-  follows:
+  Subsequently, we shall introduce specific categories of names. Roughly
+  speaking these correspond to logical entities as follows:
 
-  \<^item> Basic names (\secref{sec:basic-name}): free and bound
-  variables.
+  \<^item> Basic names (\secref{sec:basic-name}): free and bound variables.
 
   \<^item> Indexed names (\secref{sec:indexname}): schematic variables.
 
-  \<^item> Long names (\secref{sec:long-name}): constants of any kind
-  (type constructors, term constants, other concepts defined in user
-  space).  Such entities are typically managed via name spaces
-  (\secref{sec:name-space}).
+  \<^item> Long names (\secref{sec:long-name}): constants of any kind (type
+  constructors, term constants, other concepts defined in user space). Such
+  entities are typically managed via name spaces (\secref{sec:name-space}).
 \<close>
 
 
 subsection \<open>Basic names \label{sec:basic-name}\<close>
 
 text \<open>
-  A \<^emph>\<open>basic name\<close> essentially consists of a single Isabelle
-  identifier.  There are conventions to mark separate classes of basic
-  names, by attaching a suffix of underscores: one underscore means
-  \<^emph>\<open>internal name\<close>, two underscores means \<^emph>\<open>Skolem name\<close>,
-  three underscores means \<^emph>\<open>internal Skolem name\<close>.
+  A \<^emph>\<open>basic name\<close> essentially consists of a single Isabelle identifier. There
+  are conventions to mark separate classes of basic names, by attaching a
+  suffix of underscores: one underscore means \<^emph>\<open>internal name\<close>, two
+  underscores means \<^emph>\<open>Skolem name\<close>, three underscores means \<^emph>\<open>internal Skolem
+  name\<close>.
 
-  For example, the basic name \<open>foo\<close> has the internal version
-  \<open>foo_\<close>, with Skolem versions \<open>foo__\<close> and \<open>foo___\<close>, respectively.
+  For example, the basic name \<open>foo\<close> has the internal version \<open>foo_\<close>, with
+  Skolem versions \<open>foo__\<close> and \<open>foo___\<close>, respectively.
 
-  These special versions provide copies of the basic name space, apart
-  from anything that normally appears in the user text.  For example,
-  system generated variables in Isar proof contexts are usually marked
-  as internal, which prevents mysterious names like \<open>xaa\<close> to
-  appear in human-readable text.
+  These special versions provide copies of the basic name space, apart from
+  anything that normally appears in the user text. For example, system
+  generated variables in Isar proof contexts are usually marked as internal,
+  which prevents mysterious names like \<open>xaa\<close> to appear in human-readable text.
 
   \<^medskip>
-  Manipulating binding scopes often requires on-the-fly
-  renamings.  A \<^emph>\<open>name context\<close> contains a collection of already
-  used names.  The \<open>declare\<close> operation adds names to the
-  context.
+  Manipulating binding scopes often requires on-the-fly renamings. A \<^emph>\<open>name
+  context\<close> contains a collection of already used names. The \<open>declare\<close>
+  operation adds names to the context.
 
-  The \<open>invents\<close> operation derives a number of fresh names from
-  a given starting point.  For example, the first three names derived
-  from \<open>a\<close> are \<open>a\<close>, \<open>b\<close>, \<open>c\<close>.
+  The \<open>invents\<close> operation derives a number of fresh names from a given
+  starting point. For example, the first three names derived from \<open>a\<close> are \<open>a\<close>,
+  \<open>b\<close>, \<open>c\<close>.
 
-  The \<open>variants\<close> operation produces fresh names by
-  incrementing tentative names as base-26 numbers (with digits \<open>a..z\<close>) until all clashes are resolved.  For example, name \<open>foo\<close> results in variants \<open>fooa\<close>, \<open>foob\<close>, \<open>fooc\<close>, \dots, \<open>fooaa\<close>, \<open>fooab\<close> etc.; each renaming
-  step picks the next unused variant from this sequence.
+  The \<open>variants\<close> operation produces fresh names by incrementing tentative
+  names as base-26 numbers (with digits \<open>a..z\<close>) until all clashes are
+  resolved. For example, name \<open>foo\<close> results in variants \<open>fooa\<close>, \<open>foob\<close>,
+  \<open>fooc\<close>, \dots, \<open>fooaa\<close>, \<open>fooab\<close> etc.; each renaming step picks the next
+  unused variant from this sequence.
 \<close>
 
 text %mlref \<open>
@@ -649,35 +630,35 @@ text %mlref \<open>
   @{index_ML Variable.names_of: "Proof.context -> Name.context"} \\
   \end{mldecls}
 
-  \<^descr> @{ML Name.internal}~\<open>name\<close> produces an internal name
-  by adding one underscore.
+  \<^descr> @{ML Name.internal}~\<open>name\<close> produces an internal name by adding one
+  underscore.
 
-  \<^descr> @{ML Name.skolem}~\<open>name\<close> produces a Skolem name by
-  adding two underscores.
+  \<^descr> @{ML Name.skolem}~\<open>name\<close> produces a Skolem name by adding two underscores.
 
-  \<^descr> Type @{ML_type Name.context} represents the context of already
-  used names; the initial value is @{ML "Name.context"}.
+  \<^descr> Type @{ML_type Name.context} represents the context of already used names;
+  the initial value is @{ML "Name.context"}.
 
-  \<^descr> @{ML Name.declare}~\<open>name\<close> enters a used name into the
-  context.
+  \<^descr> @{ML Name.declare}~\<open>name\<close> enters a used name into the context.
 
-  \<^descr> @{ML Name.invent}~\<open>context name n\<close> produces \<open>n\<close> fresh names derived from \<open>name\<close>.
+  \<^descr> @{ML Name.invent}~\<open>context name n\<close> produces \<open>n\<close> fresh names derived from
+  \<open>name\<close>.
 
-  \<^descr> @{ML Name.variant}~\<open>name context\<close> produces a fresh
-  variant of \<open>name\<close>; the result is declared to the context.
+  \<^descr> @{ML Name.variant}~\<open>name context\<close> produces a fresh variant of \<open>name\<close>; the
+  result is declared to the context.
 
-  \<^descr> @{ML Variable.names_of}~\<open>ctxt\<close> retrieves the context
-  of declared type and term variable names.  Projecting a proof
-  context down to a primitive name context is occasionally useful when
-  invoking lower-level operations.  Regular management of ``fresh
-  variables'' is done by suitable operations of structure @{ML_structure
-  Variable}, which is also able to provide an official status of
-  ``locally fixed variable'' within the logical environment (cf.\
-  \secref{sec:variables}).
+  \<^descr> @{ML Variable.names_of}~\<open>ctxt\<close> retrieves the context of declared type and
+  term variable names. Projecting a proof context down to a primitive name
+  context is occasionally useful when invoking lower-level operations. Regular
+  management of ``fresh variables'' is done by suitable operations of
+  structure @{ML_structure Variable}, which is also able to provide an
+  official status of ``locally fixed variable'' within the logical environment
+  (cf.\ \secref{sec:variables}).
 \<close>
 
-text %mlex \<open>The following simple examples demonstrate how to produce
-  fresh names from the initial @{ML Name.context}.\<close>
+text %mlex \<open>
+  The following simple examples demonstrate how to produce fresh names from
+  the initial @{ML Name.context}.
+\<close>
 
 ML_val \<open>
   val list1 = Name.invent Name.context "a" 5;
@@ -712,36 +693,32 @@ end
 subsection \<open>Indexed names \label{sec:indexname}\<close>
 
 text \<open>
-  An \<^emph>\<open>indexed name\<close> (or \<open>indexname\<close>) is a pair of a basic
-  name and a natural number.  This representation allows efficient
-  renaming by incrementing the second component only.  The canonical
-  way to rename two collections of indexnames apart from each other is
-  this: determine the maximum index \<open>maxidx\<close> of the first
-  collection, then increment all indexes of the second collection by
-  \<open>maxidx + 1\<close>; the maximum index of an empty collection is
+  An \<^emph>\<open>indexed name\<close> (or \<open>indexname\<close>) is a pair of a basic name and a natural
+  number. This representation allows efficient renaming by incrementing the
+  second component only. The canonical way to rename two collections of
+  indexnames apart from each other is this: determine the maximum index
+  \<open>maxidx\<close> of the first collection, then increment all indexes of the second
+  collection by \<open>maxidx + 1\<close>; the maximum index of an empty collection is
   \<open>-1\<close>.
 
-  Occasionally, basic names are injected into the same pair type of
-  indexed names: then \<open>(x, -1)\<close> is used to encode the basic
-  name \<open>x\<close>.
+  Occasionally, basic names are injected into the same pair type of indexed
+  names: then \<open>(x, -1)\<close> is used to encode the basic name \<open>x\<close>.
 
   \<^medskip>
-  Isabelle syntax observes the following rules for
-  representing an indexname \<open>(x, i)\<close> as a packed string:
+  Isabelle syntax observes the following rules for representing an indexname
+  \<open>(x, i)\<close> as a packed string:
 
-  \<^item> \<open>?x\<close> if \<open>x\<close> does not end with a digit and \<open>i = 0\<close>,
+    \<^item> \<open>?x\<close> if \<open>x\<close> does not end with a digit and \<open>i = 0\<close>,
 
-  \<^item> \<open>?xi\<close> if \<open>x\<close> does not end with a digit,
+    \<^item> \<open>?xi\<close> if \<open>x\<close> does not end with a digit,
 
-  \<^item> \<open>?x.i\<close> otherwise.
+    \<^item> \<open>?x.i\<close> otherwise.
 
-
-  Indexnames may acquire large index numbers after several maxidx
-  shifts have been applied.  Results are usually normalized towards
-  \<open>0\<close> at certain checkpoints, notably at the end of a proof.
-  This works by producing variants of the corresponding basic name
-  components.  For example, the collection \<open>?x1, ?x7, ?x42\<close>
-  becomes \<open>?x, ?xa, ?xb\<close>.
+  Indexnames may acquire large index numbers after several maxidx shifts have
+  been applied. Results are usually normalized towards \<open>0\<close> at certain
+  checkpoints, notably at the end of a proof. This works by producing variants
+  of the corresponding basic name components. For example, the collection
+  \<open>?x1, ?x7, ?x42\<close> becomes \<open>?x, ?xa, ?xb\<close>.
 \<close>
 
 text %mlref \<open>
@@ -749,36 +726,34 @@ text %mlref \<open>
   @{index_ML_type indexname: "string * int"} \\
   \end{mldecls}
 
-  \<^descr> Type @{ML_type indexname} represents indexed names.  This is
-  an abbreviation for @{ML_type "string * int"}.  The second component
-  is usually non-negative, except for situations where \<open>(x,
-  -1)\<close> is used to inject basic names into this type.  Other negative
-  indexes should not be used.
+  \<^descr> Type @{ML_type indexname} represents indexed names. This is an
+  abbreviation for @{ML_type "string * int"}. The second component is usually
+  non-negative, except for situations where \<open>(x, -1)\<close> is used to inject basic
+  names into this type. Other negative indexes should not be used.
 \<close>
 
 
 subsection \<open>Long names \label{sec:long-name}\<close>
 
-text \<open>A \<^emph>\<open>long name\<close> consists of a sequence of non-empty name
-  components.  The packed representation uses a dot as separator, as
-  in ``\<open>A.b.c\<close>''.  The last component is called \<^emph>\<open>base
-  name\<close>, the remaining prefix is called \<^emph>\<open>qualifier\<close> (which may be
-  empty).  The qualifier can be understood as the access path to the
-  named entity while passing through some nested block-structure,
-  although our free-form long names do not really enforce any strict
-  discipline.
+text \<open>
+  A \<^emph>\<open>long name\<close> consists of a sequence of non-empty name components. The
+  packed representation uses a dot as separator, as in ``\<open>A.b.c\<close>''. The last
+  component is called \<^emph>\<open>base name\<close>, the remaining prefix is called
+  \<^emph>\<open>qualifier\<close> (which may be empty). The qualifier can be understood as the
+  access path to the named entity while passing through some nested
+  block-structure, although our free-form long names do not really enforce any
+  strict discipline.
 
-  For example, an item named ``\<open>A.b.c\<close>'' may be understood as
-  a local entity \<open>c\<close>, within a local structure \<open>b\<close>,
-  within a global structure \<open>A\<close>.  In practice, long names
-  usually represent 1--3 levels of qualification.  User ML code should
-  not make any assumptions about the particular structure of long
+  For example, an item named ``\<open>A.b.c\<close>'' may be understood as a local entity
+  \<open>c\<close>, within a local structure \<open>b\<close>, within a global structure \<open>A\<close>. In
+  practice, long names usually represent 1--3 levels of qualification. User ML
+  code should not make any assumptions about the particular structure of long
   names!
 
-  The empty name is commonly used as an indication of unnamed
-  entities, or entities that are not entered into the corresponding
-  name space, whenever this makes any sense.  The basic operations on
-  long names map empty names again to empty names.
+  The empty name is commonly used as an indication of unnamed entities, or
+  entities that are not entered into the corresponding name space, whenever
+  this makes any sense. The basic operations on long names map empty names
+  again to empty names.
 \<close>
 
 text %mlref \<open>
@@ -790,45 +765,42 @@ text %mlref \<open>
   @{index_ML Long_Name.explode: "string -> string list"} \\
   \end{mldecls}
 
-  \<^descr> @{ML Long_Name.base_name}~\<open>name\<close> returns the base name
-  of a long name.
+  \<^descr> @{ML Long_Name.base_name}~\<open>name\<close> returns the base name of a long name.
 
-  \<^descr> @{ML Long_Name.qualifier}~\<open>name\<close> returns the qualifier
-  of a long name.
+  \<^descr> @{ML Long_Name.qualifier}~\<open>name\<close> returns the qualifier of a long name.
 
-  \<^descr> @{ML Long_Name.append}~\<open>name\<^sub>1 name\<^sub>2\<close> appends two long
+  \<^descr> @{ML Long_Name.append}~\<open>name\<^sub>1 name\<^sub>2\<close> appends two long names.
+
+  \<^descr> @{ML Long_Name.implode}~\<open>names\<close> and @{ML Long_Name.explode}~\<open>name\<close> convert
+  between the packed string representation and the explicit list form of long
   names.
-
-  \<^descr> @{ML Long_Name.implode}~\<open>names\<close> and @{ML
-  Long_Name.explode}~\<open>name\<close> convert between the packed string
-  representation and the explicit list form of long names.
 \<close>
 
 
 subsection \<open>Name spaces \label{sec:name-space}\<close>
 
-text \<open>A \<open>name space\<close> manages a collection of long names,
-  together with a mapping between partially qualified external names
-  and fully qualified internal names (in both directions).  Note that
-  the corresponding \<open>intern\<close> and \<open>extern\<close> operations
-  are mostly used for parsing and printing only!  The \<open>declare\<close> operation augments a name space according to the accesses
+text \<open>
+  A \<open>name space\<close> manages a collection of long names, together with a mapping
+  between partially qualified external names and fully qualified internal
+  names (in both directions). Note that the corresponding \<open>intern\<close> and
+  \<open>extern\<close> operations are mostly used for parsing and printing only! The
+  \<open>declare\<close> operation augments a name space according to the accesses
   determined by a given binding, and a naming policy from the context.
 
   \<^medskip>
-  A \<open>binding\<close> specifies details about the prospective
-  long name of a newly introduced formal entity.  It consists of a
-  base name, prefixes for qualification (separate ones for system
-  infrastructure and user-space mechanisms), a slot for the original
-  source position, and some additional flags.
+  A \<open>binding\<close> specifies details about the prospective long name of a newly
+  introduced formal entity. It consists of a base name, prefixes for
+  qualification (separate ones for system infrastructure and user-space
+  mechanisms), a slot for the original source position, and some additional
+  flags.
 
   \<^medskip>
-  A \<open>naming\<close> provides some additional details for
-  producing a long name from a binding.  Normally, the naming is
-  implicit in the theory or proof context.  The \<open>full\<close>
-  operation (and its variants for different context types) produces a
-  fully qualified internal name to be entered into a name space.  The
-  main equation of this ``chemical reaction'' when binding new
-  entities in a context is as follows:
+  A \<open>naming\<close> provides some additional details for producing a long name from a
+  binding. Normally, the naming is implicit in the theory or proof context.
+  The \<open>full\<close> operation (and its variants for different context types) produces
+  a fully qualified internal name to be entered into a name space. The main
+  equation of this ``chemical reaction'' when binding new entities in a
+  context is as follows:
 
   \<^medskip>
   \begin{tabular}{l}
@@ -836,21 +808,20 @@ text \<open>A \<open>name space\<close> manages a collection of long names,
   \end{tabular}
 
   \<^bigskip>
-  As a general principle, there is a separate name space for
-  each kind of formal entity, e.g.\ fact, logical constant, type
-  constructor, type class.  It is usually clear from the occurrence in
-  concrete syntax (or from the scope) which kind of entity a name
-  refers to.  For example, the very same name \<open>c\<close> may be used
-  uniformly for a constant, type constructor, and type class.
+  As a general principle, there is a separate name space for each kind of
+  formal entity, e.g.\ fact, logical constant, type constructor, type class.
+  It is usually clear from the occurrence in concrete syntax (or from the
+  scope) which kind of entity a name refers to. For example, the very same
+  name \<open>c\<close> may be used uniformly for a constant, type constructor, and type
+  class.
 
-  There are common schemes to name derived entities systematically
-  according to the name of the main logical entity involved, e.g.\
-  fact \<open>c.intro\<close> for a canonical introduction rule related to
-  constant \<open>c\<close>.  This technique of mapping names from one
-  space into another requires some care in order to avoid conflicts.
-  In particular, theorem names derived from a type constructor or type
-  class should get an additional suffix in addition to the usual
-  qualification.  This leads to the following conventions for derived
+  There are common schemes to name derived entities systematically according
+  to the name of the main logical entity involved, e.g.\ fact \<open>c.intro\<close> for a
+  canonical introduction rule related to constant \<open>c\<close>. This technique of
+  mapping names from one space into another requires some care in order to
+  avoid conflicts. In particular, theorem names derived from a type
+  constructor or type class should get an additional suffix in addition to the
+  usual qualification. This leads to the following conventions for derived
   names:
 
   \<^medskip>
@@ -889,81 +860,76 @@ text %mlref \<open>
   @{index_ML Name_Space.is_concealed: "Name_Space.T -> string -> bool"}
   \end{mldecls}
 
-  \<^descr> Type @{ML_type binding} represents the abstract concept of
-  name bindings.
+  \<^descr> Type @{ML_type binding} represents the abstract concept of name bindings.
 
   \<^descr> @{ML Binding.empty} is the empty binding.
 
-  \<^descr> @{ML Binding.name}~\<open>name\<close> produces a binding with base
-  name \<open>name\<close>.  Note that this lacks proper source position
-  information; see also the ML antiquotation @{ML_antiquotation
-  binding}.
+  \<^descr> @{ML Binding.name}~\<open>name\<close> produces a binding with base name \<open>name\<close>. Note
+  that this lacks proper source position information; see also the ML
+  antiquotation @{ML_antiquotation binding}.
 
-  \<^descr> @{ML Binding.qualify}~\<open>mandatory name binding\<close>
-  prefixes qualifier \<open>name\<close> to \<open>binding\<close>.  The \<open>mandatory\<close> flag tells if this name component always needs to be
-  given in name space accesses --- this is mostly \<open>false\<close> in
-  practice.  Note that this part of qualification is typically used in
-  derived specification mechanisms.
+  \<^descr> @{ML Binding.qualify}~\<open>mandatory name binding\<close> prefixes qualifier \<open>name\<close>
+  to \<open>binding\<close>. The \<open>mandatory\<close> flag tells if this name component always needs
+  to be given in name space accesses --- this is mostly \<open>false\<close> in practice.
+  Note that this part of qualification is typically used in derived
+  specification mechanisms.
 
-  \<^descr> @{ML Binding.prefix} is similar to @{ML Binding.qualify}, but
-  affects the system prefix.  This part of extra qualification is
-  typically used in the infrastructure for modular specifications,
-  notably ``local theory targets'' (see also \chref{ch:local-theory}).
+  \<^descr> @{ML Binding.prefix} is similar to @{ML Binding.qualify}, but affects the
+  system prefix. This part of extra qualification is typically used in the
+  infrastructure for modular specifications, notably ``local theory targets''
+  (see also \chref{ch:local-theory}).
 
-  \<^descr> @{ML Binding.concealed}~\<open>binding\<close> indicates that the
-  binding shall refer to an entity that serves foundational purposes
-  only.  This flag helps to mark implementation details of
-  specification mechanism etc.  Other tools should not depend on the
-  particulars of concealed entities (cf.\ @{ML
+  \<^descr> @{ML Binding.concealed}~\<open>binding\<close> indicates that the binding shall refer
+  to an entity that serves foundational purposes only. This flag helps to mark
+  implementation details of specification mechanism etc. Other tools should
+  not depend on the particulars of concealed entities (cf.\ @{ML
   Name_Space.is_concealed}).
 
-  \<^descr> @{ML Binding.print}~\<open>binding\<close> produces a string
-  representation for human-readable output, together with some formal
-  markup that might get used in GUI front-ends, for example.
+  \<^descr> @{ML Binding.print}~\<open>binding\<close> produces a string representation for
+  human-readable output, together with some formal markup that might get used
+  in GUI front-ends, for example.
 
-  \<^descr> Type @{ML_type Name_Space.naming} represents the abstract
-  concept of a naming policy.
+  \<^descr> Type @{ML_type Name_Space.naming} represents the abstract concept of a
+  naming policy.
 
-  \<^descr> @{ML Name_Space.global_naming} is the default naming policy: it is
-  global and lacks any path prefix.  In a regular theory context this is
-  augmented by a path prefix consisting of the theory name.
+  \<^descr> @{ML Name_Space.global_naming} is the default naming policy: it is global
+  and lacks any path prefix. In a regular theory context this is augmented by
+  a path prefix consisting of the theory name.
 
-  \<^descr> @{ML Name_Space.add_path}~\<open>path naming\<close> augments the
-  naming policy by extending its path component.
+  \<^descr> @{ML Name_Space.add_path}~\<open>path naming\<close> augments the naming policy by
+  extending its path component.
 
-  \<^descr> @{ML Name_Space.full_name}~\<open>naming binding\<close> turns a
-  name binding (usually a basic name) into the fully qualified
-  internal name, according to the given naming policy.
+  \<^descr> @{ML Name_Space.full_name}~\<open>naming binding\<close> turns a name binding (usually
+  a basic name) into the fully qualified internal name, according to the given
+  naming policy.
 
   \<^descr> Type @{ML_type Name_Space.T} represents name spaces.
 
-  \<^descr> @{ML Name_Space.empty}~\<open>kind\<close> and @{ML Name_Space.merge}~\<open>(space\<^sub>1, space\<^sub>2)\<close> are the canonical operations for
-  maintaining name spaces according to theory data management
-  (\secref{sec:context-data}); \<open>kind\<close> is a formal comment
-  to characterize the purpose of a name space.
+  \<^descr> @{ML Name_Space.empty}~\<open>kind\<close> and @{ML Name_Space.merge}~\<open>(space\<^sub>1,
+  space\<^sub>2)\<close> are the canonical operations for maintaining name spaces according
+  to theory data management (\secref{sec:context-data}); \<open>kind\<close> is a formal
+  comment to characterize the purpose of a name space.
 
-  \<^descr> @{ML Name_Space.declare}~\<open>context strict binding
-  space\<close> enters a name binding as fully qualified internal name into
-  the name space, using the naming of the context.
+  \<^descr> @{ML Name_Space.declare}~\<open>context strict binding space\<close> enters a name
+  binding as fully qualified internal name into the name space, using the
+  naming of the context.
 
-  \<^descr> @{ML Name_Space.intern}~\<open>space name\<close> internalizes a
-  (partially qualified) external name.
+  \<^descr> @{ML Name_Space.intern}~\<open>space name\<close> internalizes a (partially qualified)
+  external name.
 
-  This operation is mostly for parsing!  Note that fully qualified
-  names stemming from declarations are produced via @{ML
-  "Name_Space.full_name"} and @{ML "Name_Space.declare"}
-  (or their derivatives for @{ML_type theory} and
+  This operation is mostly for parsing! Note that fully qualified names
+  stemming from declarations are produced via @{ML "Name_Space.full_name"} and
+  @{ML "Name_Space.declare"} (or their derivatives for @{ML_type theory} and
   @{ML_type Proof.context}).
 
-  \<^descr> @{ML Name_Space.extern}~\<open>ctxt space name\<close> externalizes a
-  (fully qualified) internal name.
+  \<^descr> @{ML Name_Space.extern}~\<open>ctxt space name\<close> externalizes a (fully qualified)
+  internal name.
 
-  This operation is mostly for printing!  User code should not rely on
-  the precise result too much.
+  This operation is mostly for printing! User code should not rely on the
+  precise result too much.
 
-  \<^descr> @{ML Name_Space.is_concealed}~\<open>space name\<close> indicates
-  whether \<open>name\<close> refers to a strictly private entity that
-  other tools are supposed to ignore!
+  \<^descr> @{ML Name_Space.is_concealed}~\<open>space name\<close> indicates whether \<open>name\<close> refers
+  to a strictly private entity that other tools are supposed to ignore!
 \<close>
 
 text %mlantiq \<open>
@@ -975,35 +941,37 @@ text %mlantiq \<open>
   @@{ML_antiquotation binding} name
   \<close>}
 
-  \<^descr> \<open>@{binding name}\<close> produces a binding with base name
-  \<open>name\<close> and the source position taken from the concrete
-  syntax of this antiquotation.  In many situations this is more
-  appropriate than the more basic @{ML Binding.name} function.
+  \<^descr> \<open>@{binding name}\<close> produces a binding with base name \<open>name\<close> and the source
+  position taken from the concrete syntax of this antiquotation. In many
+  situations this is more appropriate than the more basic @{ML Binding.name}
+  function.
 \<close>
 
-text %mlex \<open>The following example yields the source position of some
-  concrete binding inlined into the text:
+text %mlex \<open>
+  The following example yields the source position of some concrete binding
+  inlined into the text:
 \<close>
 
 ML_val \<open>Binding.pos_of @{binding here}\<close>
 
 text \<open>
   \<^medskip>
-  That position can be also printed in a message as follows:\<close>
+  That position can be also printed in a message as follows:
+\<close>
 
 ML_command
   \<open>writeln
     ("Look here" ^ Position.here (Binding.pos_of @{binding here}))\<close>
 
-text \<open>This illustrates a key virtue of formalized bindings as
-  opposed to raw specifications of base names: the system can use this
-  additional information for feedback given to the user (error
-  messages etc.).
+text \<open>
+  This illustrates a key virtue of formalized bindings as opposed to raw
+  specifications of base names: the system can use this additional information
+  for feedback given to the user (error messages etc.).
 
   \<^medskip>
-  The following example refers to its source position
-  directly, which is occasionally useful for experimentation and
-  diagnostic purposes:\<close>
+  The following example refers to its source position directly, which is
+  occasionally useful for experimentation and diagnostic purposes:
+\<close>
 
 ML_command \<open>warning ("Look here" ^ Position.here @{here})\<close>
 
