src/Doc/Implementation/Isar.thy
@@ -6,60 +6,57 @@ begin
 
 chapter \<open>Isar language elements\<close>
 
-text \<open>The Isar proof language (see also
-  @{cite \<open>\S2\<close> "isabelle-isar-ref"}) consists of three main categories of
-  language elements:
+text \<open>
+  The Isar proof language (see also @{cite \<open>\S2\<close> "isabelle-isar-ref"})
+  consists of three main categories of language elements:
 
-  \<^enum> Proof \<^emph>\<open>commands\<close> define the primary language of
-  transactions of the underlying Isar/VM interpreter.  Typical
-  examples are @{command "fix"}, @{command "assume"}, @{command
-  "show"}, @{command "proof"}, and @{command "qed"}.
+  \<^enum> Proof \<^emph>\<open>commands\<close> define the primary language of transactions of the
+  underlying Isar/VM interpreter. Typical examples are @{command "fix"},
+  @{command "assume"}, @{command "show"}, @{command "proof"}, and @{command
+  "qed"}.
 
-  Composing proof commands according to the rules of the Isar/VM leads
-  to expressions of structured proof text, such that both the machine
-  and the human reader can give it a meaning as formal reasoning.
+  Composing proof commands according to the rules of the Isar/VM leads to
+  expressions of structured proof text, such that both the machine and the
+  human reader can give it a meaning as formal reasoning.
 
-  \<^enum> Proof \<^emph>\<open>methods\<close> define a secondary language of mixed
-  forward-backward refinement steps involving facts and goals.
-  Typical examples are @{method rule}, @{method unfold}, and @{method
-  simp}.
+  \<^enum> Proof \<^emph>\<open>methods\<close> define a secondary language of mixed forward-backward
+  refinement steps involving facts and goals. Typical examples are @{method
+  rule}, @{method unfold}, and @{method simp}.
 
-  Methods can occur in certain well-defined parts of the Isar proof
-  language, say as arguments to @{command "proof"}, @{command "qed"},
-  or @{command "by"}.
+  Methods can occur in certain well-defined parts of the Isar proof language,
+  say as arguments to @{command "proof"}, @{command "qed"}, or @{command
+  "by"}.
 
-  \<^enum> \<^emph>\<open>Attributes\<close> define a tertiary language of small
-  annotations to theorems being defined or referenced.  Attributes can
-  modify both the context and the theorem.
+  \<^enum> \<^emph>\<open>Attributes\<close> define a tertiary language of small annotations to theorems
+  being defined or referenced. Attributes can modify both the context and the
+  theorem.
 
-  Typical examples are @{attribute intro} (which affects the context),
-  and @{attribute symmetric} (which affects the theorem).
+  Typical examples are @{attribute intro} (which affects the context), and
+  @{attribute symmetric} (which affects the theorem).
 \<close>
 
 
 section \<open>Proof commands\<close>
 
-text \<open>A \<^emph>\<open>proof command\<close> is state transition of the Isar/VM
-  proof interpreter.
+text \<open>
+  A \<^emph>\<open>proof command\<close> is state transition of the Isar/VM proof interpreter.
 
-  In principle, Isar proof commands could be defined in user-space as
-  well.  The system is built like that in the first place: one part of
-  the commands are primitive, the other part is defined as derived
-  elements.  Adding to the genuine structured proof language requires
-  profound understanding of the Isar/VM machinery, though, so this is
-  beyond the scope of this manual.
+  In principle, Isar proof commands could be defined in user-space as well.
+  The system is built like that in the first place: one part of the commands
+  are primitive, the other part is defined as derived elements. Adding to the
+  genuine structured proof language requires profound understanding of the
+  Isar/VM machinery, though, so this is beyond the scope of this manual.
 
-  What can be done realistically is to define some diagnostic commands
-  that inspect the general state of the Isar/VM, and report some
-  feedback to the user.  Typically this involves checking of the
-  linguistic \<^emph>\<open>mode\<close> of a proof state, or peeking at the pending
-  goals (if available).
+  What can be done realistically is to define some diagnostic commands that
+  inspect the general state of the Isar/VM, and report some feedback to the
+  user. Typically this involves checking of the linguistic \<^emph>\<open>mode\<close> of a proof
+  state, or peeking at the pending goals (if available).
 
-  Another common application is to define a toplevel command that
-  poses a problem to the user as Isar proof state and processes the
-  final result relatively to the context.  Thus a proof can be
-  incorporated into the context of some user-space tool, without
-  modifying the Isar proof language itself.\<close>
+  Another common application is to define a toplevel command that poses a
+  problem to the user as Isar proof state and processes the final result
+  relatively to the context. Thus a proof can be incorporated into the context
+  of some user-space tool, without modifying the Isar proof language itself.
+\<close>
 
 text %mlref \<open>
   \begin{mldecls}
@@ -77,61 +74,56 @@ text %mlref \<open>
   (term * term list) list list -> Proof.context -> Proof.state"} \\
   \end{mldecls}
 
-  \<^descr> Type @{ML_type Proof.state} represents Isar proof states.
-  This is a block-structured configuration with proof context,
-  linguistic mode, and optional goal.  The latter consists of goal
-  context, goal facts (``\<open>using\<close>''), and tactical goal state
-  (see \secref{sec:tactical-goals}).
+  \<^descr> Type @{ML_type Proof.state} represents Isar proof states. This is a
+  block-structured configuration with proof context, linguistic mode, and
+  optional goal. The latter consists of goal context, goal facts
+  (``\<open>using\<close>''), and tactical goal state (see \secref{sec:tactical-goals}).
 
-  The general idea is that the facts shall contribute to the
-  refinement of some parts of the tactical goal --- how exactly is
-  defined by the proof method that is applied in that situation.
+  The general idea is that the facts shall contribute to the refinement of
+  some parts of the tactical goal --- how exactly is defined by the proof
+  method that is applied in that situation.
 
   \<^descr> @{ML Proof.assert_forward}, @{ML Proof.assert_chain}, @{ML
-  Proof.assert_backward} are partial identity functions that fail
-  unless a certain linguistic mode is active, namely ``\<open>proof(state)\<close>'', ``\<open>proof(chain)\<close>'', ``\<open>proof(prove)\<close>'', respectively (using the terminology of
-  @{cite "isabelle-isar-ref"}).
+  Proof.assert_backward} are partial identity functions that fail unless a
+  certain linguistic mode is active, namely ``\<open>proof(state)\<close>'',
+  ``\<open>proof(chain)\<close>'', ``\<open>proof(prove)\<close>'', respectively (using the terminology
+  of @{cite "isabelle-isar-ref"}).
 
-  It is advisable study the implementations of existing proof commands
-  for suitable modes to be asserted.
+  It is advisable study the implementations of existing proof commands for
+  suitable modes to be asserted.
 
-  \<^descr> @{ML Proof.simple_goal}~\<open>state\<close> returns the structured
-  Isar goal (if available) in the form seen by ``simple'' methods
-  (like @{method simp} or @{method blast}).  The Isar goal facts are
-  already inserted as premises into the subgoals, which are presented
-  individually as in @{ML Proof.goal}.
+  \<^descr> @{ML Proof.simple_goal}~\<open>state\<close> returns the structured Isar goal (if
+  available) in the form seen by ``simple'' methods (like @{method simp} or
+  @{method blast}). The Isar goal facts are already inserted as premises into
+  the subgoals, which are presented individually as in @{ML Proof.goal}.
 
-  \<^descr> @{ML Proof.goal}~\<open>state\<close> returns the structured Isar
-  goal (if available) in the form seen by regular methods (like
-  @{method rule}).  The auxiliary internal encoding of Pure
-  conjunctions is split into individual subgoals as usual.
+  \<^descr> @{ML Proof.goal}~\<open>state\<close> returns the structured Isar goal (if available)
+  in the form seen by regular methods (like @{method rule}). The auxiliary
+  internal encoding of Pure conjunctions is split into individual subgoals as
+  usual.
 
-  \<^descr> @{ML Proof.raw_goal}~\<open>state\<close> returns the structured
-  Isar goal (if available) in the raw internal form seen by ``raw''
-  methods (like @{method induct}).  This form is rarely appropriate
-  for diagnostic tools; @{ML Proof.simple_goal} or @{ML Proof.goal}
-  should be used in most situations.
+  \<^descr> @{ML Proof.raw_goal}~\<open>state\<close> returns the structured Isar goal (if
+  available) in the raw internal form seen by ``raw'' methods (like @{method
+  induct}). This form is rarely appropriate for diagnostic tools; @{ML
+  Proof.simple_goal} or @{ML Proof.goal} should be used in most situations.
 
-  \<^descr> @{ML Proof.theorem}~\<open>before_qed after_qed statement ctxt\<close>
-  initializes a toplevel Isar proof state within a given context.
+  \<^descr> @{ML Proof.theorem}~\<open>before_qed after_qed statement ctxt\<close> initializes a
+  toplevel Isar proof state within a given context.
 
-  The optional \<open>before_qed\<close> method is applied at the end of
-  the proof, just before extracting the result (this feature is rarely
-  used).
+  The optional \<open>before_qed\<close> method is applied at the end of the proof, just
+  before extracting the result (this feature is rarely used).
 
-  The \<open>after_qed\<close> continuation receives the extracted result
-  in order to apply it to the final context in a suitable way (e.g.\
-  storing named facts).  Note that at this generic level the target
-  context is specified as @{ML_type Proof.context}, but the usual
-  wrapping of toplevel proofs into command transactions will provide a
-  @{ML_type local_theory} here (\chref{ch:local-theory}).  This
-  affects the way how results are stored.
+  The \<open>after_qed\<close> continuation receives the extracted result in order to apply
+  it to the final context in a suitable way (e.g.\ storing named facts). Note
+  that at this generic level the target context is specified as @{ML_type
+  Proof.context}, but the usual wrapping of toplevel proofs into command
+  transactions will provide a @{ML_type local_theory} here
+  (\chref{ch:local-theory}). This affects the way how results are stored.
 
-  The \<open>statement\<close> is given as a nested list of terms, each
-  associated with optional @{keyword "is"} patterns as usual in the
-  Isar source language.  The original nested list structure over terms
-  is turned into one over theorems when \<open>after_qed\<close> is
-  invoked.
+  The \<open>statement\<close> is given as a nested list of terms, each associated with
+  optional @{keyword "is"} patterns as usual in the Isar source language. The
+  original nested list structure over terms is turned into one over theorems
+  when \<open>after_qed\<close> is invoked.
 \<close>
 
 
@@ -140,15 +132,16 @@ text %mlantiq \<open>
   @{ML_antiquotation_def "Isar.goal"} & : & \<open>ML_antiquotation\<close> \\
   \end{matharray}
 
-  \<^descr> \<open>@{Isar.goal}\<close> refers to the regular goal state (if
-  available) of the current proof state managed by the Isar toplevel
-  --- as abstract value.
+  \<^descr> \<open>@{Isar.goal}\<close> refers to the regular goal state (if available) of the
+  current proof state managed by the Isar toplevel --- as abstract value.
 
-  This only works for diagnostic ML commands, such as @{command
-  ML_val} or @{command ML_command}.
+  This only works for diagnostic ML commands, such as @{command ML_val} or
+  @{command ML_command}.
 \<close>
 
-text %mlex \<open>The following example peeks at a certain goal configuration.\<close>
+text %mlex \<open>
+  The following example peeks at a certain goal configuration.
+\<close>
 
 notepad
 begin
@@ -159,8 +152,10 @@ begin
     sorry
 end
 
-text \<open>Here we see 3 individual subgoals in the same way as regular
-  proof methods would do.\<close>
+text \<open>
+  Here we see 3 individual subgoals in the same way as regular proof methods
+  would do.
+\<close>
 
 
 section \<open>Proof methods\<close>
@@ -172,42 +167,38 @@ text \<open>
   normal circumstances, the goal context remains unchanged, but it is also
   possible to declare named extensions of the proof context (\<^emph>\<open>cases\<close>).
 
-  This means a proof method is like a structurally enhanced tactic
-  (cf.\ \secref{sec:tactics}).  The well-formedness conditions for
-  tactics need to hold for methods accordingly, with the following
-  additions.
+  This means a proof method is like a structurally enhanced tactic (cf.\
+  \secref{sec:tactics}). The well-formedness conditions for tactics need to
+  hold for methods accordingly, with the following additions.
 
-  \<^item> Goal addressing is further limited either to operate
-  uniformly on \<^emph>\<open>all\<close> subgoals, or specifically on the
-  \<^emph>\<open>first\<close> subgoal.
+  \<^item> Goal addressing is further limited either to operate uniformly on \<^emph>\<open>all\<close>
+  subgoals, or specifically on the \<^emph>\<open>first\<close> subgoal.
 
-  Exception: old-style tactic emulations that are embedded into the
-  method space, e.g.\ @{method rule_tac}.
+  Exception: old-style tactic emulations that are embedded into the method
+  space, e.g.\ @{method rule_tac}.
 
-  \<^item> A non-trivial method always needs to make progress: an
-  identical follow-up goal state has to be avoided.\<^footnote>\<open>This
-  enables the user to write method expressions like \<open>meth\<^sup>+\<close>
-  without looping, while the trivial do-nothing case can be recovered
-  via \<open>meth\<^sup>?\<close>.\<close>
+  \<^item> A non-trivial method always needs to make progress: an identical follow-up
+  goal state has to be avoided.\<^footnote>\<open>This enables the user to write method
+  expressions like \<open>meth\<^sup>+\<close> without looping, while the trivial do-nothing case
+  can be recovered via \<open>meth\<^sup>?\<close>.\<close>
 
-  Exception: trivial stuttering steps, such as ``@{method -}'' or
-  @{method succeed}.
+  Exception: trivial stuttering steps, such as ``@{method -}'' or @{method
+  succeed}.
 
-  \<^item> Goal facts passed to the method must not be ignored.  If there
-  is no sensible use of facts outside the goal state, facts should be
-  inserted into the subgoals that are addressed by the method.
+  \<^item> Goal facts passed to the method must not be ignored. If there is no
+  sensible use of facts outside the goal state, facts should be inserted into
+  the subgoals that are addressed by the method.
 
 
   \<^medskip>
-  Syntactically, the language of proof methods appears as
-  arguments to Isar commands like @{command "by"} or @{command apply}.
-  User-space additions are reasonably easy by plugging suitable
-  method-valued parser functions into the framework, using the
-  @{command method_setup} command, for example.
+  Syntactically, the language of proof methods appears as arguments to Isar
+  commands like @{command "by"} or @{command apply}. User-space additions are
+  reasonably easy by plugging suitable method-valued parser functions into the
+  framework, using the @{command method_setup} command, for example.
 
   To get a better idea about the range of possibilities, consider the
-  following Isar proof schemes.  This is the general form of
-  structured proof text:
+  following Isar proof schemes. This is the general form of structured proof
+  text:
 
   \<^medskip>
   \begin{tabular}{l}
@@ -218,11 +209,12 @@ text \<open>
   \end{tabular}
   \<^medskip>
 
-  The goal configuration consists of \<open>facts\<^sub>1\<close> and
-  \<open>facts\<^sub>2\<close> appended in that order, and various \<open>props\<close> being claimed.  The \<open>initial_method\<close> is invoked
-  with facts and goals together and refines the problem to something
-  that is handled recursively in the proof \<open>body\<close>.  The \<open>terminal_method\<close> has another chance to finish any remaining
-  subgoals, but it does not see the facts of the initial step.
+  The goal configuration consists of \<open>facts\<^sub>1\<close> and \<open>facts\<^sub>2\<close> appended in that
+  order, and various \<open>props\<close> being claimed. The \<open>initial_method\<close> is invoked
+  with facts and goals together and refines the problem to something that is
+  handled recursively in the proof \<open>body\<close>. The \<open>terminal_method\<close> has another
+  chance to finish any remaining subgoals, but it does not see the facts of
+  the initial step.
 
   \<^medskip>
   This pattern illustrates unstructured proof scripts:
@@ -237,51 +229,48 @@ text \<open>
   \end{tabular}
   \<^medskip>
 
-  The \<open>method\<^sub>1\<close> operates on the original claim while
-  using \<open>facts\<^sub>1\<close>.  Since the @{command apply} command
-  structurally resets the facts, the \<open>method\<^sub>2\<close> will
-  operate on the remaining goal state without facts.  The \<open>method\<^sub>3\<close> will see again a collection of \<open>facts\<^sub>3\<close> that has been inserted into the script explicitly.
+  The \<open>method\<^sub>1\<close> operates on the original claim while using \<open>facts\<^sub>1\<close>. Since
+  the @{command apply} command structurally resets the facts, the \<open>method\<^sub>2\<close>
+  will operate on the remaining goal state without facts. The \<open>method\<^sub>3\<close> will
+  see again a collection of \<open>facts\<^sub>3\<close> that has been inserted into the script
+  explicitly.
 
   \<^medskip>
-  Empirically, any Isar proof method can be categorized as
-  follows.
+  Empirically, any Isar proof method can be categorized as follows.
 
-  \<^enum> \<^emph>\<open>Special method with cases\<close> with named context additions
-  associated with the follow-up goal state.
+    \<^enum> \<^emph>\<open>Special method with cases\<close> with named context additions associated
+    with the follow-up goal state.
 
-  Example: @{method "induct"}, which is also a ``raw'' method since it
-  operates on the internal representation of simultaneous claims as
-  Pure conjunction (\secref{sec:logic-aux}), instead of separate
-  subgoals (\secref{sec:tactical-goals}).
+    Example: @{method "induct"}, which is also a ``raw'' method since it
+    operates on the internal representation of simultaneous claims as Pure
+    conjunction (\secref{sec:logic-aux}), instead of separate subgoals
+    (\secref{sec:tactical-goals}).
 
-  \<^enum> \<^emph>\<open>Structured method\<close> with strong emphasis on facts outside
-  the goal state.
+    \<^enum> \<^emph>\<open>Structured method\<close> with strong emphasis on facts outside the goal
+    state.
 
-  Example: @{method "rule"}, which captures the key ideas behind
-  structured reasoning in Isar in its purest form.
+    Example: @{method "rule"}, which captures the key ideas behind structured
+    reasoning in Isar in its purest form.
 
-  \<^enum> \<^emph>\<open>Simple method\<close> with weaker emphasis on facts, which are
-  inserted into subgoals to emulate old-style tactical ``premises''.
+    \<^enum> \<^emph>\<open>Simple method\<close> with weaker emphasis on facts, which are inserted into
+    subgoals to emulate old-style tactical ``premises''.
 
-  Examples: @{method "simp"}, @{method "blast"}, @{method "auto"}.
+    Examples: @{method "simp"}, @{method "blast"}, @{method "auto"}.
 
-  \<^enum> \<^emph>\<open>Old-style tactic emulation\<close> with detailed numeric goal
-  addressing and explicit references to entities of the internal goal
-  state (which are otherwise invisible from proper Isar proof text).
-  The naming convention \<open>foo_tac\<close> makes this special
-  non-standard status clear.
+    \<^enum> \<^emph>\<open>Old-style tactic emulation\<close> with detailed numeric goal addressing and
+    explicit references to entities of the internal goal state (which are
+    otherwise invisible from proper Isar proof text). The naming convention
+    \<open>foo_tac\<close> makes this special non-standard status clear.
 
-  Example: @{method "rule_tac"}.
-
+    Example: @{method "rule_tac"}.
 
   When implementing proof methods, it is advisable to study existing
-  implementations carefully and imitate the typical ``boiler plate''
-  for context-sensitive parsing and further combinators to wrap-up
-  tactic expressions as methods.\<^footnote>\<open>Aliases or abbreviations of
-  the standard method combinators should be avoided.  Note that from
-  Isabelle99 until Isabelle2009 the system did provide various odd
-  combinations of method syntax wrappers that made applications more
-  complicated than necessary.\<close>
+  implementations carefully and imitate the typical ``boiler plate'' for
+  context-sensitive parsing and further combinators to wrap-up tactic
+  expressions as methods.\<^footnote>\<open>Aliases or abbreviations of the standard method
+  combinators should be avoided. Note that from Isabelle99 until Isabelle2009
+  the system did provide various odd combinations of method syntax wrappers
+  that made applications more complicated than necessary.\<close>
 \<close>
 
 text %mlref \<open>
@@ -296,8 +285,7 @@ text %mlref \<open>
   string -> theory -> theory"} \\
   \end{mldecls}
 
-  \<^descr> Type @{ML_type Proof.method} represents proof methods as
-  abstract type.
+  \<^descr> Type @{ML_type Proof.method} represents proof methods as abstract type.
 
   \<^descr> @{ML CONTEXT_METHOD}~\<open>(fn facts => context_tactic)\<close> wraps \<open>context_tactic\<close>
   depending on goal facts as a general proof method that may change the proof
@@ -305,36 +293,36 @@ text %mlref \<open>
   Proof_Context.update_cases}, which is wrapped up as combinator @{index_ML
   CONTEXT_CASES} for convenience.
 
-  \<^descr> @{ML METHOD}~\<open>(fn facts => tactic)\<close> wraps \<open>tactic\<close> depending on goal facts as regular proof method; the goal
-  context is passed via method syntax.
+  \<^descr> @{ML METHOD}~\<open>(fn facts => tactic)\<close> wraps \<open>tactic\<close> depending on goal facts
+  as regular proof method; the goal context is passed via method syntax.
 
-  \<^descr> @{ML SIMPLE_METHOD}~\<open>tactic\<close> wraps a tactic that
-  addresses all subgoals uniformly as simple proof method.  Goal facts
-  are already inserted into all subgoals before \<open>tactic\<close> is
-  applied.
+  \<^descr> @{ML SIMPLE_METHOD}~\<open>tactic\<close> wraps a tactic that addresses all subgoals
+  uniformly as simple proof method. Goal facts are already inserted into all
+  subgoals before \<open>tactic\<close> is applied.
 
-  \<^descr> @{ML SIMPLE_METHOD'}~\<open>tactic\<close> wraps a tactic that
-  addresses a specific subgoal as simple proof method that operates on
-  subgoal 1.  Goal facts are inserted into the subgoal then the \<open>tactic\<close> is applied.
+  \<^descr> @{ML SIMPLE_METHOD'}~\<open>tactic\<close> wraps a tactic that addresses a specific
+  subgoal as simple proof method that operates on subgoal 1. Goal facts are
+  inserted into the subgoal then the \<open>tactic\<close> is applied.
 
-  \<^descr> @{ML Method.insert_tac}~\<open>ctxt facts i\<close> inserts \<open>facts\<close> into subgoal \<open>i\<close>.  This is convenient to reproduce
-  part of the @{ML SIMPLE_METHOD} or @{ML SIMPLE_METHOD'} wrapping
-  within regular @{ML METHOD}, for example.
+  \<^descr> @{ML Method.insert_tac}~\<open>ctxt facts i\<close> inserts \<open>facts\<close> into subgoal \<open>i\<close>.
+  This is convenient to reproduce part of the @{ML SIMPLE_METHOD} or @{ML
+  SIMPLE_METHOD'} wrapping within regular @{ML METHOD}, for example.
 
-  \<^descr> @{ML Method.setup}~\<open>name parser description\<close> provides
-  the functionality of the Isar command @{command method_setup} as ML
-  function.
+  \<^descr> @{ML Method.setup}~\<open>name parser description\<close> provides the functionality of
+  the Isar command @{command method_setup} as ML function.
 \<close>
 
-text %mlex \<open>See also @{command method_setup} in
-  @{cite "isabelle-isar-ref"} which includes some abstract examples.
+text %mlex \<open>
+  See also @{command method_setup} in @{cite "isabelle-isar-ref"} which
+  includes some abstract examples.
 
   \<^medskip>
-  The following toy examples illustrate how the goal facts
-  and state are passed to proof methods.  The predefined proof method
-  called ``@{method tactic}'' wraps ML source of type @{ML_type
-  tactic} (abstracted over @{ML_text facts}).  This allows immediate
-  experimentation without parsing of concrete syntax.\<close>
+  The following toy examples illustrate how the goal facts and state are
+  passed to proof methods. The predefined proof method called ``@{method
+  tactic}'' wraps ML source of type @{ML_type tactic} (abstracted over
+  @{ML_text facts}). This allows immediate experimentation without parsing of
+  concrete syntax.
+\<close>
 
 notepad
 begin
@@ -357,8 +345,9 @@ end
 
 text \<open>
   \<^medskip>
-  The next example implements a method that simplifies
-  the first subgoal by rewrite rules that are given as arguments.\<close>
+  The next example implements a method that simplifies the first subgoal by
+  rewrite rules that are given as arguments.
+\<close>
 
 method_setup my_simp =
   \<open>Attrib.thms >> (fn thms => fn ctxt =>
@@ -367,21 +356,21 @@ method_setup my_simp =
         (put_simpset HOL_basic_ss ctxt addsimps thms) i)))\<close>
   "rewrite subgoal by given rules"
 
-text \<open>The concrete syntax wrapping of @{command method_setup} always
-  passes-through the proof context at the end of parsing, but it is
-  not used in this example.
+text \<open>
+  The concrete syntax wrapping of @{command method_setup} always
+  passes-through the proof context at the end of parsing, but it is not used
+  in this example.
 
-  The @{ML Attrib.thms} parser produces a list of theorems from the
-  usual Isar syntax involving attribute expressions etc.\ (syntax
-  category @{syntax thmrefs}) @{cite "isabelle-isar-ref"}.  The resulting
-  @{ML_text thms} are added to @{ML HOL_basic_ss} which already
-  contains the basic Simplifier setup for HOL.
+  The @{ML Attrib.thms} parser produces a list of theorems from the usual Isar
+  syntax involving attribute expressions etc.\ (syntax category @{syntax
+  thmrefs}) @{cite "isabelle-isar-ref"}. The resulting @{ML_text thms} are
+  added to @{ML HOL_basic_ss} which already contains the basic Simplifier
+  setup for HOL.
 
-  The tactic @{ML asm_full_simp_tac} is the one that is also used in
-  method @{method simp} by default.  The extra wrapping by the @{ML
-  CHANGED} tactical ensures progress of simplification: identical goal
-  states are filtered out explicitly to make the raw tactic conform to
-  standard Isar method behaviour.
+  The tactic @{ML asm_full_simp_tac} is the one that is also used in method
+  @{method simp} by default. The extra wrapping by the @{ML CHANGED} tactical
+  ensures progress of simplification: identical goal states are filtered out
+  explicitly to make the raw tactic conform to standard Isar method behaviour.
 
   \<^medskip>
   Method @{method my_simp} can be used in Isar proofs like this:
@@ -395,8 +384,9 @@ begin
   have "a = c" by (my_simp a b)
 end
 
-text \<open>Here is a similar method that operates on all subgoals,
-  instead of just the first one.\<close>
+text \<open>
+  Here is a similar method that operates on all subgoals, instead of just the
+  first one.\<close>
 
 method_setup my_simp_all =
   \<open>Attrib.thms >> (fn thms => fn ctxt =>
@@ -416,15 +406,18 @@ end
 
 text \<open>
   \<^medskip>
-  Apart from explicit arguments, common proof methods
-  typically work with a default configuration provided by the context. As a
-  shortcut to rule management we use a cheap solution via the @{command
-  named_theorems} command to declare a dynamic fact in the context.\<close>
+  Apart from explicit arguments, common proof methods typically work with a
+  default configuration provided by the context. As a shortcut to rule
+  management we use a cheap solution via the @{command named_theorems} command
+  to declare a dynamic fact in the context.
+\<close>
 
 named_theorems my_simp
 
-text \<open>The proof method is now defined as before, but we append the
-  explicit arguments and the rules from the context.\<close>
+text \<open>
+  The proof method is now defined as before, but we append the explicit
+  arguments and the rules from the context.
+\<close>
 
 method_setup my_simp' =
   \<open>Attrib.thms >> (fn thms => fn ctxt =>
@@ -440,8 +433,7 @@ method_setup my_simp' =
 
 text \<open>
   \<^medskip>
-  Method @{method my_simp'} can be used in Isar proofs
-  like this:
+  Method @{method my_simp'} can be used in Isar proofs like this:
 \<close>
 
 notepad
@@ -454,60 +446,58 @@ end
 
 text \<open>
   \<^medskip>
-  The @{method my_simp} variants defined above are
-  ``simple'' methods, i.e.\ the goal facts are merely inserted as goal
-  premises by the @{ML SIMPLE_METHOD'} or @{ML SIMPLE_METHOD} wrapper.
-  For proof methods that are similar to the standard collection of
-  @{method simp}, @{method blast}, @{method fast}, @{method auto}
-  there is little more that can be done.
+  The @{method my_simp} variants defined above are ``simple'' methods, i.e.\
+  the goal facts are merely inserted as goal premises by the @{ML
+  SIMPLE_METHOD'} or @{ML SIMPLE_METHOD} wrapper. For proof methods that are
+  similar to the standard collection of @{method simp}, @{method blast},
+  @{method fast}, @{method auto} there is little more that can be done.
 
-  Note that using the primary goal facts in the same manner as the
-  method arguments obtained via concrete syntax or the context does
-  not meet the requirement of ``strong emphasis on facts'' of regular
-  proof methods, because rewrite rules as used above can be easily
-  ignored.  A proof text ``@{command using}~\<open>foo\<close>~@{command
-  "by"}~\<open>my_simp\<close>'' where \<open>foo\<close> is not used would
-  deceive the reader.
+  Note that using the primary goal facts in the same manner as the method
+  arguments obtained via concrete syntax or the context does not meet the
+  requirement of ``strong emphasis on facts'' of regular proof methods,
+  because rewrite rules as used above can be easily ignored. A proof text
+  ``@{command using}~\<open>foo\<close>~@{command "by"}~\<open>my_simp\<close>'' where \<open>foo\<close> is not used
+  would deceive the reader.
 
   \<^medskip>
-  The technical treatment of rules from the context requires
-  further attention.  Above we rebuild a fresh @{ML_type simpset} from
-  the arguments and \<^emph>\<open>all\<close> rules retrieved from the context on
-  every invocation of the method.  This does not scale to really large
-  collections of rules, which easily emerges in the context of a big
-  theory library, for example.
+  The technical treatment of rules from the context requires further
+  attention. Above we rebuild a fresh @{ML_type simpset} from the arguments
+  and \<^emph>\<open>all\<close> rules retrieved from the context on every invocation of the
+  method. This does not scale to really large collections of rules, which
+  easily emerges in the context of a big theory library, for example.
 
   This is an inherent limitation of the simplistic rule management via
-  @{command named_theorems}, because it lacks tool-specific
-  storage and retrieval.  More realistic applications require
-  efficient index-structures that organize theorems in a customized
-  manner, such as a discrimination net that is indexed by the
-  left-hand sides of rewrite rules.  For variations on the Simplifier,
-  re-use of the existing type @{ML_type simpset} is adequate, but
-  scalability would require it be maintained statically within the
-  context data, not dynamically on each tool invocation.\<close>
+  @{command named_theorems}, because it lacks tool-specific storage and
+  retrieval. More realistic applications require efficient index-structures
+  that organize theorems in a customized manner, such as a discrimination net
+  that is indexed by the left-hand sides of rewrite rules. For variations on
+  the Simplifier, re-use of the existing type @{ML_type simpset} is adequate,
+  but scalability would require it be maintained statically within the context
+  data, not dynamically on each tool invocation.
+\<close>
 
 
 section \<open>Attributes \label{sec:attributes}\<close>
 
-text \<open>An \<^emph>\<open>attribute\<close> is a function \<open>context \<times> thm \<rightarrow>
-  context \<times> thm\<close>, which means both a (generic) context and a theorem
-  can be modified simultaneously.  In practice this mixed form is very
-  rare, instead attributes are presented either as \<^emph>\<open>declaration
-  attribute:\<close> \<open>thm \<rightarrow> context \<rightarrow> context\<close> or \<^emph>\<open>rule
+text \<open>
+  An \<^emph>\<open>attribute\<close> is a function \<open>context \<times> thm \<rightarrow> context \<times> thm\<close>, which means
+  both a (generic) context and a theorem can be modified simultaneously. In
+  practice this mixed form is very rare, instead attributes are presented
+  either as \<^emph>\<open>declaration attribute:\<close> \<open>thm \<rightarrow> context \<rightarrow> context\<close> or \<^emph>\<open>rule
   attribute:\<close> \<open>context \<rightarrow> thm \<rightarrow> thm\<close>.
 
-  Attributes can have additional arguments via concrete syntax.  There
-  is a collection of context-sensitive parsers for various logical
-  entities (types, terms, theorems).  These already take care of
-  applying morphisms to the arguments when attribute expressions are
-  moved into a different context (see also \secref{sec:morphisms}).
+  Attributes can have additional arguments via concrete syntax. There is a
+  collection of context-sensitive parsers for various logical entities (types,
+  terms, theorems). These already take care of applying morphisms to the
+  arguments when attribute expressions are moved into a different context (see
+  also \secref{sec:morphisms}).
 
-  When implementing declaration attributes, it is important to operate
-  exactly on the variant of the generic context that is provided by
-  the system, which is either global theory context or local proof
-  context.  In particular, the background theory of a local context
-  must not be modified in this situation!\<close>
+  When implementing declaration attributes, it is important to operate exactly
+  on the variant of the generic context that is provided by the system, which
+  is either global theory context or local proof context. In particular, the
+  background theory of a local context must not be modified in this
+  situation!
+\<close>
 
 text %mlref \<open>
   \begin{mldecls}
@@ -520,8 +510,7 @@ text %mlref \<open>
   string -> theory -> theory"} \\
   \end{mldecls}
 
-  \<^descr> Type @{ML_type attribute} represents attributes as concrete
-  type alias.
+  \<^descr> Type @{ML_type attribute} represents attributes as concrete type alias.
 
   \<^descr> @{ML Thm.rule_attribute}~\<open>thms (fn context => rule)\<close> wraps a
   context-dependent rule (mapping on @{ML_type thm}) as attribute.
@@ -537,9 +526,8 @@ text %mlref \<open>
   When forming an abstract closure, the system may provide a dummy fact as
   \<open>thm\<close>. In that case, \<open>decl\<close> is bypassed.
 
-  \<^descr> @{ML Attrib.setup}~\<open>name parser description\<close> provides
-  the functionality of the Isar command @{command attribute_setup} as
-  ML function.
+  \<^descr> @{ML Attrib.setup}~\<open>name parser description\<close> provides the functionality of
+  the Isar command @{command attribute_setup} as ML function.
 \<close>
 
 text %mlantiq \<open>
@@ -551,15 +539,16 @@ text %mlantiq \<open>
   @@{ML_antiquotation attributes} attributes
   \<close>}
 
-  \<^descr> \<open>@{attributes [\<dots>]}\<close> embeds attribute source
-  representation into the ML text, which is particularly useful with
-  declarations like @{ML Local_Theory.note}.  Attribute names are
-  internalized at compile time, but the source is unevaluated.  This
-  means attributes with formal arguments (types, terms, theorems) may
-  be subject to odd effects of dynamic scoping!
+  \<^descr> \<open>@{attributes [\<dots>]}\<close> embeds attribute source representation into the ML
+  text, which is particularly useful with declarations like @{ML
+  Local_Theory.note}. Attribute names are internalized at compile time, but
+  the source is unevaluated. This means attributes with formal arguments
+  (types, terms, theorems) may be subject to odd effects of dynamic scoping!
 \<close>
 
-text %mlex \<open>See also @{command attribute_setup} in
-  @{cite "isabelle-isar-ref"} which includes some abstract examples.\<close>
+text %mlex \<open>
+  See also @{command attribute_setup} in @{cite "isabelle-isar-ref"} which
+  includes some abstract examples.
+\<close>
 
 end
